### 1.
```prolog
{
{tier(drache)},
{tier(maus)},
{tier(katze)},
{tier(hund)},

{jagt(drache, hund)},
{jagt(drache, katze)},
{jagt(hund, katze)},
{jagt(katze, maus)},
{jagt(adler, maus)},
{jagt(schlange, maus)},
{jagt(drache, hund)},
{jagt(hund, katze)},
{jagt(adler, schlange)},
{jagt(drache, adler)},

% beute(X) :- tier(X), jagt(_, X).
{beute(x), ¬tier(X), ¬jagt(Y, X)},

% jaeger(X) :- jagt(X, _), not(jagt(_, X)).

{jaeger(X), ¬jagt(X, Y), jagt(Z, X)}

% beute_und_jaeger(X) :- jagt(X, _), jagt(_, X).
{beute_und_jaeger(X), ¬jagt(X, Y), ¬jagt(Z, X)}
}

?{¬beute_und_jaeger(katze)}

```
2: Anfrage 1
?- beute_und_jaeger(katze).
- {¬beute_und_jaeger(katze)}
- {¬jagt(X, Y), ¬jagt(Z, X), beute_und_jaeger(X)}
- {¬jagt(katze, Y), ¬jagt(Z, katze)}   

Faktenprüfung:
- jagt(katze, maus) -> ¬jagt(katze, Y) ist falsch
- jagt(hund, katze) -> ¬jagt(Z, katze) ist falsch

?- beute_und_jaeger(katze). -> true.

Anfrage 2: 
?- beute(X).
- {¬beute(X)}
- {¬tier(X), ¬jagt(Y, X), beute(X)}
- {¬tier(X), ¬jagt(Y, X)}

Versuch mit X = maus:
- tier(maus) ∈ Basis
- jagt(katze, maus) ∈ Basis ⇒ jagt(Y, maus) ist erfüllbar

X=maus


```prolog

tier(drache).
tier(maus).
tier(katze).
tier(hund).

jagt(drache, hund).
jagt(drache, katze).
jagt(hund, katze).
jagt(katze, maus).

beute(X) :- tier(X), jagt(_, X).
jaeger(X) :- jagt(X, _), \+ jagt(_, X).
beute_und_jaeger(X) :- jagt(X, _), jagt(_, X).

:- initialization(main).

main :-
  % (beute_und_jaeger(katze) -> write('=> TRUE') ; write('=> FALSE')).
  (beute(X), write(X), false ; true).
```